Changed to big-step evaluation for expressions

Sympaths.v
@@ -187,6 +187,8 @@ Module SymPaths.
   | APlus a1 a2 => (aeval st a1) + (aeval st a2)
   | AMult a1 a2 => (aeval st a1) * (aeval st a2)
   end.
+  Compute (aeval (X !-> 1) (X + 1 + (3 * X))).
+  Compute (aeval empty_st 2). 
 
   Fixpoint beval (st : state) (b : bexpr) : bool :=
     match b with
@@ -208,201 +210,11 @@ Module SymPaths.
   Compute aeval ( X !-> 2 ; Y !-> 3 ; empty_st) (X + Y)%expr.
   Compute beval ( X !-> 2 ; Y !-> 5 ; empty_st) (X < Y)%expr.
 
-  (*
-  Reserved Notation "st '=[' c ']=>' st'"
-                  (at level 40).
-
-  (**This version has the normal while *)
-  Inductive ceval_relation : statements -> state -> state -> Prop :=
-  | E_Skip : forall st,
-      st =[ skip ]=> st
-  | E_Ass  : forall st a1 n l,
-      aeval st a1 = n ->
-      st =[ l ::= a1 ]=> (l !-> n ; st)
-  | E_Seq : forall s1 s2 st st' st'',
-      st  =[ s1 ]=> st'  ->
-      st' =[ s2 ]=> st'' ->
-      st  =[ s1 ;; s2 ]=> st''                                          
-  | E_IfTrue : forall st st' cond s1 s2,
-      beval st cond = true ->
-      st =[ s1 ]=> st' ->
-      st =[ If cond THEN s1 ELSE s2 ]=> st'
-  | E_IfFalse : forall st st' cond s1 s2,
-      beval st cond = false ->
-      st =[ s2 ]=> st' ->
-      st =[ If cond THEN s1 ELSE s2 ]=> st'
-  | E_WhileFalse : forall cond st s,
-      beval st cond = false ->
-      st =[ WHILE cond DO s END ]=> st
-  | E_WhileTrue : forall st st' st'' cond s,
-      beval st cond = true ->
-      st  =[ s ]=> st' ->
-      st' =[ WHILE cond DO s END ]=> st'' ->
-       st  =[ WHILE cond DO s END ]=> st''
-  (*| E_WhilenFalse : forall cond st s n,
-      beval st cond = false ->
-      st =[ WHILE cond FOR n DO s END ]=> st
-  | E_Whilen0 : forall cond st s n,
-      n = 0 ->
-      st =[ WHILE cond FOR n DO s END ]=> st                                      
-  | E_WhilenTrue : forall st st' st'' cond s n,
-      beval st cond = true ->
-      st  =[ s ]=> st' ->
-      st' =[ WHILE cond FOR n DO s END ]=> st'' -> (*where can we decrement n???*)
-      st  =[ WHILE cond FOR n-1 DO s END ]=> st'' *)
-                                                                        
-  where "st =[ s ]=> st'" := (ceval_relation s st st').
-
-  (* Definition test_nwhile : statements := 
-     (WHILE ~(Z = 0) FOR 2 DO
-       Z ::= Z + 1
-                   END)%stm. *)
-   
-  (* Example ceval_rel_while:
-     (Z !-> 1) =[ test_nwhile ]=> (Z !->3; Z !-> 2; Z !-> 1).
-   Proof.
-     unfold test_nwhile. apply E_WhilenTrue. -> fails here *)
-
-  
-  Check empty_st =[ (X ::= 1) ]=> (X !-> 1).
-
-  Example ceval_skip :
-    empty_st =[ skip ]=> empty_st.
-  Proof.
-    apply E_Skip. Qed. 
-
-    
-  Example ceval_relation_ex1:
-    empty_st =[ (X ::= 1) ]=> (X !-> 1).
-  Proof.
-    apply E_Ass. simpl. reflexivity.
-  Qed.
-
-  Example ceval_relation_ex2:
-    (X !-> 1) =[ (Y ::= 3) ]=> ( Y !-> 3 ; X !-> 1).
-  Proof.
-    apply E_Ass. reflexivity. Qed. 
-
-  Example ceval_relation_ex3:
-    empty_st =[ (X ::= 1 ) ;; (Y ::= 3) ]=> ( Y !-> 3; X !-> 1).
-  Proof.
-    eapply E_Seq. apply E_Ass. reflexivity.
-    -apply E_Ass. reflexivity. Qed. 
-
-  Example ceval_relation_ex4:
-    empty_st =[
-      X ::= 1 ;;
-      If X < 1
-         THEN Y ::= 3
-         ELSE Z ::= 5
-    ]=> ( Z !->5 ;  X !-> 1  ).
-  Proof.
-    eapply E_Seq.
-    - apply E_Ass. reflexivity.
-    - apply E_IfFalse. reflexivity.
-      apply E_Ass. reflexivity. Qed.
-
-  Example ceval_relation_ex5:
-    empty_st =[
-      X ::= 0 ;;
-      WHILE (X < 1) DO
-            X ::= X + 1
-                        END ]=> (X !-> 1 ; X !-> 0 ).
-  Proof.
-    eapply E_Seq. apply E_Ass. reflexivity.
-    -eapply E_WhileTrue. reflexivity.
-     *apply E_Ass. simpl. reflexivity.
-     *apply E_WhileFalse. simpl. reflexivity. Qed.
-
-  Theorem cevalR_deterministic : forall s st st1 st2,
-      st =[ s ]=> st1 ->
-      st =[ s ]=> st2 ->
-      st1 = st2. 
-  Proof.
-    intros. generalize dependent st2. induction H.
-    -intros. inversion H0.  (* what do we need for thisto be true *) reflexivity.
-    - intros. inversion H0. assert (n0 = n). rewrite H in H5. symmetry in H5. assumption.
-      rewrite H6 . reflexivity.
-    - intros. inversion H1. assert (st' = st'0). apply IHceval_relation1 in H4. assumption. rewrite <- H8 in H7. apply IHceval_relation2 in H7. assumption.
-    - intros. inversion H1. apply IHceval_relation in H8. assumption. rewrite H in H7. discriminate H7.
-    - intros. inversion H1. rewrite H in H7. discriminate H7. apply IHceval_relation in H8. assumption.
-    - intros. inversion H0. reflexivity. rewrite H in H3. discriminate H3.
-    - intros. inversion H2. rewrite <- H6 in H7. rewrite H in H7. discriminate H7.
-      assert (st'0 = st'). apply IHceval_relation1 in H6. symmetry in H6. assumption.  rewrite H10 in H9. apply IHceval_relation2 in H9. assumption. Qed. *)
-
-
   (*Single-step (can add multi-step) evaluation -> what we need for Threads!*)
   Inductive aval : aexpr -> Prop :=
   | av_num : forall n, aval (ANum n).
   
-  Reserved Notation " t '/' st '-->a' t' " (at level 40, st at level 39).
-  Inductive astep : state -> aexpr -> aexpr -> Prop :=
-  | AS_Var : forall st i,
-      AVar i / st -->a ANum (st i)
-  | AS_Plus1 : forall st a1 a1' a2,
-      a1 / st -->a a1' ->
-      (APlus a1 a2) / st -->a (APlus a1' a2)
-  | AS_Plus2 : forall st v a2 a2',
-      aval v ->
-      a2 / st -->a a2' ->
-      (APlus v a2) / st -->a (APlus v a2')
-  | AS_Plus : forall st n1 n2,
-      APlus (ANum n1) (ANum n2) / st -->a ANum (n1 + n2)
-  | AS_Mult1 : forall st a1 a1' a2,
-      a1 / st -->a a1' ->
-      (APlus a1 a2) / st -->a (APlus a1' a2)
-  | AS_Mult2 : forall st v a2 a2',
-      aval v ->
-      a2 / st -->a a2' ->
-      (APlus v a2) / st -->a (APlus v a2')
-  | A_Mult : forall st n1 n2,
-      AMult (ANum n1) (ANum n2) / st -->a ANum (n1 * n2)
-  where " t '/' st '-->a' t' " := (astep st t t').
-
-  Reserved Notation " t '/' st '-->b' t' " (at level 40, st at level 39).
-  Inductive bstep : state -> bexpr -> bexpr -> Prop :=
-  | BS_NotStep : forall st b1 b1',
-      b1 / st -->b b1' ->
-      (BNot b1) /st -->b (BNot b1')
-  | BS_NotTrue : forall st,
-      (BNot BTrue) / st -->b BFalse
-  | BS_NotFalse : forall st,
-      (BNot BFalse) / st -->b BTrue
-  | BS_AndStep : forall st b1 b1' b2,
-      b1 / st -->b b1' ->
-      (BAnd b1 b2) / st -->b (BAnd b1' b2)
-  | BS_AndTrueStep : forall st b2 b2',
-      b2 / st -->b b2' ->
-      (BAnd BTrue b2) / st -->b (BAnd BTrue b2')
-  | BS_AndTrueTrue : forall st,
-      (BAnd BTrue BTrue) / st -->b BTrue
-  | BS_AndTrueFalse : forall st,
-      (BAnd BTrue BFalse) / st -->b BFalse
-  | BS_AndFalse : forall st b2,
-      (BAnd BFalse b2) / st -->b BFalse
-  | BS_Eq1 : forall st a1 a1' a2,
-      a1 / st -->a a1' ->
-      (BEq a1 a2) / st -->b (BEq a1' a2)
-  | BS_Eq2 : forall st v a2 a2',
-      aval v ->
-      a2 / st -->a a2' ->
-      (BEq v a2) / st -->b (BEq v a2')
-  | BS_Eq : forall st n1 n2,
-      (BEq (ANum n1) (ANum n2)) / st -->b
-                                (if (n1 =? n2) then BTrue else BFalse)
-  | BS_Lt1 : forall st a1 a1' a2,
-      a1 / st -->a a1' ->
-      (BLessThan a1 a2) / st -->b (BLessThan a1' a2)
-  | BS_Lt2 : forall st v a2 a2',
-      aval v ->
-      a2 / st -->a a2' ->
-      (BLessThan v a2) / st -->b (BLessThan v a2')
-  | BS_Lt : forall st n1 n2,
-      (BLessThan (ANum n1) (ANum n2)) / st -->b
-                                      (if (n1 <? n2) then BTrue else BFalse)
-  where " t '/' st '-->b' t' " := (bstep st t t').
-
-  (*For the evaluation of statements we will use SKIP to know when we reach the end of the executiom aka
+  (*For the evaluation of statements we will use SKIP to know when we reach the end of the execution aka
  have reached normal form *)
   (*The while statement is the most interesting one, we use If stm , transform the while into a 
   conditional followed by the same WHILE *)
@@ -410,9 +222,8 @@ Module SymPaths.
    Open Scope stm_scope.
     Reserved Notation " t '/' st '-->' t' '/' st' " (at level 40, st at level 39, t' at level 39).
     Inductive cstep : (statements * state) -> (statements * state) -> Prop :=
-    | CS_AssStep : forall st i a a',
-        a / st -->a a' ->
-        (i ::= a ) / st --> (i ::= a') / st
+    | CS_AssStep : forall st i a,
+        (i ::= a ) / st --> (i ::= (aeval st a)) / st
     | CS_Ass : forall st i n,
         (i ::= (ANum n)) / st --> (skip) / (i !-> n ; st) 
     | CS_SeqStep : forall st s1 s1' s2 st',
@@ -420,9 +231,8 @@ Module SymPaths.
         (s1 ;; s2) / st --> (s1' ;; s2) / st'
     | CS_SeqFinish : forall st s2,
         (skip ;; s2) / st --> s2 / st 
-    | CS_IfStep : forall st b b' s1 s2,
-        b / st -->b b' ->
-        (If b THEN s1 ELSE s2) / st --> (If b' THEN s1 ELSE s2) / st
+    | CS_IfStep : forall st b s1 s2,
+        (If b THEN s1 ELSE s2) / st --> (If (beval st b) THEN s1 ELSE s2) / st
     | CS_IfTrue : forall st s1 s2,
         (If BTrue THEN s1 ELSE s2) / st --> s1 / st
     | CS_IfFalse : forall st s1 s2,
@@ -433,36 +243,6 @@ Module SymPaths.
                            (*this could be a good place to reduce n*) 
     where " t '/' st '-->' t' '/' st' " := (cstep (t,st) (t',st')).  
 
-    Inductive threadPool : Type :=
-    | Thread (s : statements)
-    | TPar (tp1 tp2: threadPool).
-
-    Coercion Thread : statements >-> threadPool.
-    Check Thread(skip).
-    Check (TPar (skip) (skip)).
-    Check (TPar (TPar (skip) (skip)) (skip)). 
-    
-    Reserved Notation " t '/' st '-->t' t' '/' st' " (at level 40, st at level 39, t' at level 39).
-    Open Scope stm_scope. 
-    Inductive tpstep : (threadPool * state) -> (threadPool * state) -> Prop :=
-    | TS_T1 : forall st t1 t1' t2 st',
-        t1 / st -->t t1' / st' ->
-        (TPar t1 t2) / st -->t (TPar t1' t2) / st'
-    | TS_T2 : forall st t1 t2 t2' st',
-        t2 / st -->t t2' / st' ->
-        (TPar t1 t2) / st -->t (TPar t1 t2') / st'
-    | TS_ST1 : forall st s1 s1' s2 st', (*when we arrive to statements*)
-        s1 / st --> s1' / st' ->
-        (TPar s1 s2) / st -->t (TPar s1' s2) / st'        
-    | TS_ST2 : forall st s1 s2 s2' st',
-        s2 / st --> s2' / st' ->
-        (TPar s1 s2) / st -->t (TPar s1 s2') / st'
-    | TS_STDone : forall st,
-        (TPar (skip) (skip)) / st -->t Thread(skip) / st
-        
-          where " t '/' st '-->t' t' '/' st' " := (tpstep (t,st) (t', st')).
-        
-   
 Definition relation (X : Type) := X -> X -> Prop.
     
 Inductive multi {X : Type} (R : relation X) : relation X :=
@@ -476,11 +256,9 @@ Definition cmultistep := multi cstep.
 
 Notation " t '/' st '-->*' t' '/' st' " :=
    (multi cstep  (t,st) (t',st'))
-   (at level 40, st at level 39, t' at level 39).
+     (at level 40, st at level 39, t' at level 39).
 
-(*Examples taken from the book*)
-
-
+(*Examples illustrating how evaluation works*)
 Example cstep_ex_skip :
   forall st,
     (skip) / st -->* (skip) / st .
@@ -511,45 +289,137 @@ Proof.
   apply multi_refl. Qed.
 
 Example cstep_ex4_if:
-    stm_if / empty_st -->* (skip) / ( Z !-> 5 ;  X !-> 1 ).
-  Proof.
-    eapply E_Seq.
-    - apply E_Ass. reflexivity.
-    - apply E_IfFalse. reflexivity.
-      apply E_Ass. reflexivity. Qed.
-
-
-    
-    
-        
-
-Definition par_loop : com :=
-  PAR
-    Y ::= 1
-  WITH
-    WHILE Y = 0 DO
-      X ::= X + 1
-    END
-    END.
-
-Example par_loop_example_0:
-  exists st',
-       par_loop / empty_st  -->* SKIP / st'
-    /\ st' X = 0.
+  stm_if / empty_st -->* (skip) / ( Z !-> 5 ;  X !-> 1 ).
 Proof.
-Remember eapply ex_intro. 
-  Admitted. *)
-                                                
+  unfold stm_if.
+  eapply multi_step. eapply CS_SeqStep. apply CS_Ass.
+  eapply multi_step. eapply CS_SeqFinish.
+  eapply multi_step. apply CS_IfStep. simpl. 
+  eapply multi_step. apply CS_IfFalse. eapply multi_step. apply CS_Ass.
+  apply multi_refl. Qed.
 
-                       
+Example cstep_ex5_while:
+  stm_while / empty_st -->* (skip) / (X !-> 1 ; X !-> 0).
+Proof.
+  unfold stm_while.
+  eapply multi_step. eapply CS_SeqStep. apply CS_Ass.
+  eapply multi_step. eapply CS_SeqFinish.
+  eapply multi_step. apply CS_While.
+  eapply multi_step. apply CS_IfStep. simpl.
+  eapply multi_step. apply CS_IfTrue. eapply multi_step. eapply CS_SeqStep.
+         apply CS_AssStep. simpl. 
+  eapply multi_step. eapply CS_SeqStep. apply CS_Ass.
+  eapply multi_step. eapply CS_SeqFinish.
+  eapply multi_step. eapply CS_While.
+  eapply multi_step. eapply CS_IfStep. simpl.  
+  eapply multi_step. eapply CS_IfFalse.
+  apply multi_refl. Qed. 
+
+ (*Adding the threads*)
+
+    Inductive threadPool : Type :=
+    | Thread (s : statements)
+    | TPar (tp1 tp2: threadPool).
+
+    Coercion Thread : statements >-> threadPool.
+    Check Thread(skip).
+    Check (TPar (skip) (skip)).
+    Check (TPar (TPar (skip) (skip)) (skip)). 
     
+    Reserved Notation " t '/' st '-->t' t' '/' st' " (at level 40, st at level 39, t' at level 39).
+    Open Scope stm_scope. 
+    Inductive tpstep : (threadPool * state) -> (threadPool * state) -> Prop :=
+    | TS_T1 : forall st t1 t1' t2 st',
+        t1 / st -->t t1' / st' ->
+        (TPar t1 t2) / st -->t (TPar t1' t2) / st'
+    | TS_T2 : forall st t1 t2 t2' st',
+        t2 / st -->t t2' / st' ->
+        (TPar t1 t2) / st -->t (TPar t1 t2') / st'
+    | TS_ST1 : forall st s1 s1' s2 st', (*when we arrive to statements*)
+        s1 / st --> s1' / st' ->
+        (TPar s1 s2) / st -->t (TPar s1' s2) / st'        
+    | TS_ST2 : forall st s1 s2 s2' st',
+        s2 / st --> s2' / st' ->
+        (TPar s1 s2) / st -->t (TPar s1 s2') / st'
+    | TS_STDone : forall st,
+        (TPar (skip) (skip)) / st -->t Thread(skip) / st
+        
+          where " t '/' st '-->t' t' '/' st' " := (tpstep (t,st) (t', st')).
+
+Definition tmultistep := multi tpstep.
+
+Notation " t '/' st '-->t*' t' '/' st' " :=
+   (multi tpstep  (t,st) (t',st'))
+     (at level 40, st at level 39, t' at level 39).
   
-  
-  
-                                
-                        
-                   
-    
+Definition stm_thread : threadPool :=
+  (TPar
+    (TPar
+      (Y ::= 1)
+      (WHILE Y = 0 DO
+          X ::= X + 1
+                      END) )
+    (Z ::= 5)).
+
+Check ex_intro.
+
+Example tpstep_ex1:
+  exists st',
+       stm_thread / empty_st  -->t* Thread(skip) / st'
+       /\ st' X = 0.
+Proof.
+  eapply ex_intro. split.
+  unfold stm_thread.
+  (*thread 1 first*)
+  eapply multi_step. apply TS_T1.
+  (*thread 1 in thread 1*)
+  apply TS_ST1. apply CS_Ass.
+
+  (*then thread 1 again*)
+  eapply multi_step. apply TS_T1.
+  (*and thread 2 in thread 1*)
+  apply TS_ST2. apply CS_While.
+  eapply multi_step. apply TS_T1. apply TS_ST2.
+      apply CS_IfStep. simpl. 
+  eapply multi_step. apply TS_T1. apply TS_ST2. apply CS_IfFalse.
+  eapply multi_step. apply TS_T1. apply TS_STDone.
+
+  (*finally we look at thread 2*)
+  eapply multi_step. apply TS_ST2. apply CS_Ass.
+  eapply multi_step. apply TS_STDone. 
+  eapply multi_refl.
+  reflexivity. Qed. 
+
+Example tpstep_ex2:
+  exists st',
+    stm_thread / empty_st -->t* Thread(skip) /  st'
+    /\ st' X = 1.
+Proof.
+  eapply ex_intro. split. unfold stm_thread. 
+  (*thread 2 first*)
+  eapply multi_step. apply TS_ST2. apply CS_Ass.
+
+  (*then tread 1*)  
+  eapply multi_step. apply TS_T1.
+  (*thread 2 in thread 1 first*)
+  apply TS_ST2. apply CS_While. 
+  eapply multi_step. apply TS_T1. apply TS_ST2. apply CS_IfStep. simpl.  
+  eapply multi_step. apply TS_T1. apply TS_ST2. apply CS_IfTrue.
+  eapply multi_step. apply TS_T1. apply TS_ST2. apply CS_SeqStep. apply CS_AssStep. simpl.
+  eapply multi_step. apply TS_T1. apply TS_ST2. apply CS_SeqStep. apply CS_Ass.
+  eapply multi_step. apply TS_T1. apply TS_ST2. apply CS_SeqFinish.
+
+  (*then thread 1 in thread 1*)
+  eapply multi_step. apply TS_T1. apply TS_ST1. apply CS_Ass.
+
+  (*finally thread 2 in thread 1 again*)
+  eapply multi_step. apply TS_T1. apply TS_ST2. apply CS_While. 
+  eapply multi_step. apply TS_T1. apply TS_ST2. apply CS_IfStep. simpl.
+  eapply multi_step. apply TS_T1. apply TS_ST2. apply CS_IfFalse.
+  eapply multi_step. apply TS_T1. apply TS_STDone.
+  eapply multi_step. apply TS_STDone.
+  apply multi_refl.
+  reflexivity. Qed.   
   
 Close Scope stm_scope.    
 End SymPaths.
